Add more annotations to casts

theories/autosubst/GAST.sig
@@ -19,7 +19,7 @@ revealP : term -> term -> term
 
 gheq : term -> term -> term -> term
 ghrefl : term -> term -> term
-ghcast : term -> term -> term -> term
+ghcast : term -> term -> term -> term -> term -> term -> term
 
 bot : term
 bot_elim : mode -> term -> term -> term
